record for weak and strong automatons

src/automatons/dAutomaton_causal.thy
@@ -6,36 +6,39 @@ begin
 
 section \<open>Deterministic Weak Automata\<close>
 
-record ('state::type, 'in, 'out, 'initOut) dAutomaton_weak  =
+record ('state::type, 'in, 'out) dAutomaton_weak  =
   dawTransition :: "('state \<Rightarrow> 'in\<^sup>\<surd> \<Rightarrow> ('state \<times> 'out\<^sup>\<surd>))"
   dawInitState :: "'state"
-  dawInitOut:: "'initOut\<^sup>\<surd>"
 
-definition daw2da::"('state::type, 'in::{chan,finite}, 'out,'initOut) dAutomaton_weak \<Rightarrow> ('state::type, 'in, 'out) dAutomaton" where
+record ('state::type,'in,'out)dAutomaton_strong = "('state::type, 'in, 'out) dAutomaton_weak" 
+                                                  + dasInitOut:: "'out\<^sup>\<surd>"
+
+definition daw2da::"('state::type, 'in::{chan,finite}, 'out) dAutomaton_weak \<Rightarrow> ('state::type, 'in, 'out) dAutomaton" where
 "daw2da \<equiv> \<lambda>aut. (| daTransition =(\<lambda>s sbe. (fst(dawTransition aut s sbe),sbe2sb (snd(dawTransition aut s sbe)))),
-                 daInitState = dawInitState(aut), daInitOut = (sbe2sb (dawInitOut aut)\<star>) |)"
+                 daInitState = dawInitState(aut), daInitOut = \<bottom> |)"
 
 subsection \<open>Weak Automaton Semantic options\<close>
 
 subsubsection \<open>Deterministic Automaton Semantic\<close>
 
-definition semantik_weak::"('state::type, 'in::{chan,finite}, 'out::chan, 'initOut) dAutomaton_weak \<Rightarrow> ('in,'out)spfw"where
+definition semantik_weak::"('state::type, 'in::{chan,finite}, 'out::chan) dAutomaton_weak \<Rightarrow> ('in,'out)spfw"where
 "semantik_weak autw = Abs_spfw(daSem(daw2da autw))"
 
 
-definition dawStateSem :: "('s::type, 'I::{finite,chan},'O,'initO) dAutomaton_weak \<Rightarrow> ('s \<Rightarrow> ('I\<^sup>\<Omega> \<rightarrow> 'O\<^sup>\<Omega>))" where
+definition dawStateSem :: "('s::type, 'I::{finite,chan},'O) dAutomaton_weak \<Rightarrow> ('s \<Rightarrow> ('I\<^sup>\<Omega> \<rightarrow> 'O\<^sup>\<Omega>))" where
 "dawStateSem da = fix\<cdot>(\<Lambda> h. (\<lambda> state. sb_case\<cdot>
                         (\<lambda>sbe. \<Lambda> sb.
                           let (nextState, output) = dawTransition da state sbe in
                             output \<bullet>\<^sup>\<surd> h nextState\<cdot>sb)
                       ))"
 
-definition dawSem :: "('s::type, 'I::{finite,chan},'O,'initO) dAutomaton_weak \<Rightarrow> ('I\<^sup>\<Omega> \<rightarrow> 'O\<^sup>\<Omega>)" where
+definition dawSem :: "('s::type, 'I::{finite,chan},'O) dAutomaton_weak \<Rightarrow> ('I\<^sup>\<Omega> \<rightarrow> 'O\<^sup>\<Omega>)" where
 "dawSem da = (\<Lambda> sb. ((dawStateSem da (dawInitState da))\<cdot>sb))"
+
 
 subsubsection \<open>Rum96 Automaton Semantic\<close>
 
-function Rum_tap::"('s::type, 'in::{chan,finite},'out,'initOut) dAutomaton_weak \<Rightarrow> ('s \<Rightarrow> ('in,'out) spfw) set" where
+function Rum_tap::"('s::type, 'in::{chan,finite},'out) dAutomaton_weak \<Rightarrow> ('s \<Rightarrow> ('in,'out) spfw) set" where
 "Rum_tap aut = {h | h. \<forall>m s. \<exists>t out . ((snd(dawTransition aut s m)) = out) \<and>
                     (\<exists>h2\<in> (Rum_tap aut). \<forall>i .
           (Rep_spfw(h s))\<cdot>(m \<bullet>\<^sup>\<surd> i) = out \<bullet>\<^sup>\<surd> ((Rep_spfw(h2 t))\<cdot>i))}"
@@ -43,30 +46,28 @@ function Rum_tap::"('s::type, 'in::{chan,finite},'out,'initOut) dAutomaton_weak 
 
 (*Termination for Rum_tap necessary?*)
 
-fun Rum_ta::"('s::type, 'in::{chan,finite},'out,'initOut) dAutomaton_weak \<Rightarrow> (('in,'out) spfw) set"where
-"Rum_ta aut = {g | g. \<exists>h\<in>(Rum_tap aut). \<exists> s (out::'initOut\<^sup>\<surd>). \<forall>i.
-              (Rep_spfw g)\<cdot>i = ((sbe2sb out)\<star>)\<bullet>\<^sup>\<Omega>((Rep_spfw(h s))\<cdot>i)}"
+fun Rum_ta::"('s::type, 'in::{chan,finite},'out) dAutomaton_weak \<Rightarrow> (('in,'out) spfw) set"where
+"Rum_ta aut = {g | g. \<exists>h\<in>(Rum_tap aut). \<exists> s (out::'out\<^sup>\<surd>). \<forall>i.
+              (Rep_spfw g)\<cdot>i = out\<bullet>\<^sup>\<surd>((Rep_spfw(h s))\<cdot>i)}"
 
 section \<open>Deterministic strong Automaton\<close>
-
-type_synonym ('s,'in,'out)dAutomaton_strong = "('s,'in,'out,'out)dAutomaton_weak"
-
 
 subsection \<open>Strong Automaton Semantic options \<close>
 
 subsubsection \<open>Deterministic Automaton Semantic\<close>
 
 definition semantik_strong::"('s::type, 'in::{finite,chan}, 'out) dAutomaton_strong \<Rightarrow> ('in,'out)spfs"where
-"semantik_strong auts = Abs_spfs(semantik_weak auts)"
+"semantik_strong auts = Abs_spfs(semantik_weak (dAutomaton_weak.truncate auts))"
+
 
 definition dasSem :: "('s::type, 'I::{finite,chan},'O) dAutomaton_strong \<Rightarrow> ('I\<^sup>\<Omega> \<rightarrow> 'O\<^sup>\<Omega>)" where
-"dasSem da = (\<Lambda> sb. (dawInitOut da) \<bullet>\<^sup>\<surd> ((dawStateSem da (dawInitState da))\<cdot>sb))"
+"dasSem da = (\<Lambda> sb. (dasInitOut da) \<bullet>\<^sup>\<surd> (dawSem (dAutomaton_weak.truncate da)\<cdot>sb))"
 
 
 subsection \<open>Rum96 Automaton Semantic \<close>
 
 fun Rum_ta_strong::"('s::type, 'in::{chan,finite},'out) dAutomaton_strong \<Rightarrow> (('in,'out) spfs) set"where
-"Rum_ta_strong aut = Abs_spfs `(Rum_ta aut)"
+"Rum_ta_strong aut = Abs_spfs `(Rum_ta (dAutomaton_weak.truncate aut))"
 
 
 subsection \<open>*Causal Sem lemmas \<close>
@@ -120,8 +121,10 @@ lemma dawstatesem_weak:
   oops
 
 lemma dassem_insert:
-  "dasSem automat\<cdot>sb = (dawInitOut automat) \<bullet>\<^sup>\<surd> ((dawStateSem automat (dawInitState automat))\<cdot>sb)"
-  by (simp add: dasSem_def)
+  "dasSem automat\<cdot>sb = (dasInitOut automat) \<bullet>\<^sup>\<surd> ((dawStateSem (dAutomaton_weak.truncate automat) (dawInitState automat))\<cdot>sb)"
+  apply (simp add: dasSem_def dawSem_def)
+  apply(subgoal_tac "dawInitState (dAutomaton_weak.truncate automat) = dawInitState automat",auto) (*Sollte gelten*)
+  sorry 
 
 lemma dassem_bottom:
   shows "dasSem automat\<cdot>\<bottom> = sbe2sb (dawInitOut automat)"
@@ -136,13 +139,10 @@ section \<open>automaton to sscanl equivalence locale\<close>
 locale sscanlGen =
   fixes daTransition::"'state::countable \<Rightarrow> 'a::countable \<Rightarrow> ('state\<times>'b::countable)"
   and   daInitialState::"'state"
-  and   daInitialOut::"'b"    (* TODO, schwach kausal = keine initiale ausgabe! *)
   and fin::"'a::countable \<Rightarrow> 'in::{chan,finite} \<Rightarrow> M"  
   and fout::"'b::countable \<Rightarrow> 'out::{chan,finite} \<Rightarrow> M"
-  and emptytype::"'c itself"
   assumes sbegenfin:"sbeGen fin"
       and sbegenfout:"sbeGen fout"
-      and emptytypeempty:"chIsEmpty emptytype"
 begin
 
 definition daTransitionH::"'state \<Rightarrow> 'in\<^sup>\<surd> \<Rightarrow> ('state \<times> 'out\<^sup>\<surd>)" where
@@ -150,12 +150,9 @@ definition daTransitionH::"'state \<Rightarrow> 'in\<^sup>\<surd> \<Rightarrow> 
   (s, sbeGen.setter fout output))"
 
 definition "da = \<lparr> dawTransition = daTransitionH,
-                 dawInitState =daInitialState, dawInitOut =  (sbeGen.setter fout daInitialOut) \<rparr>"
+                 dawInitState =daInitialState \<rparr>"
 
-definition "(daw::('state, 'in, 'out, 'c) dAutomaton_weak) = \<lparr> dawTransition = daTransitionH,
-                 dawInitState =daInitialState, dawInitOut =  Abs_sbElem(None)\<rparr>"
-
-lemma daut2sscanl:"dawStateSem daw state\<cdot>(input::'in\<^sup>\<Omega>) = 
+lemma daut2sscanl:"dawStateSem daw state\<cdot>(input::'in\<^sup>\<Omega>) =
        sbeGen.setterSB fout\<cdot>(sscanlAsnd daTransition state\<cdot>(sbeGen.getterSB fin\<cdot>input))"
 proof(induction input)
   case adm
@@ -195,12 +192,10 @@ section \<open>automaton to smap equivalence locale\<close>
 locale smapGen =
   fixes daTransition::"'state::countable \<Rightarrow> 'a::countable \<Rightarrow> ('state\<times>'b::countable)"
   and   daInitialState::"'state"
-  and   daInitialOut::"'b"    (* TODO, schwach kausal = keine initiale ausgabe! *)
   and fin::"'a::countable \<Rightarrow> 'in::{chan,finite} \<Rightarrow> M"  
   and fout::"'b::countable \<Rightarrow> 'out::{chan,finite} \<Rightarrow> M"
-  and emptytype::"'c itself"
   and loopState::"'state"
-  assumes scscanlgenf:"sscanlGen fin fout emptytype"
+  assumes scscanlgenf:"sscanlGen fin fout"
   and singlestate:"\<And>sbe. fst(daTransition loopState sbe) = loopState"
 begin
 
@@ -212,7 +207,7 @@ shows"sscanlAsnd f s = smap g"
   apply(rule cfun_eqI)
   by(induct_tac x rule: ind,simp_all add: assms)
 
-lemma daut2smap:"dawStateSem (sscanlGen.daw daTransition daInitialState fin fout) loopState\<cdot>(input::'in\<^sup>\<Omega>) = 
+lemma daut2smap:"dawStateSem (sscanlGen.da daTransition daInitialState fin fout) loopState\<cdot>(input::'in\<^sup>\<Omega>) = 
        sbeGen.setterSB fout\<cdot>(smap (\<lambda>e. snd(daTransition loopState e))\<cdot>(sbeGen.getterSB fin\<cdot>input))"
   apply(subst sscanlGen.daut2sscanl)(*
   using scscanlgenf sscanlGen.sbegenfin apply auto[1]
